asset/final/spec/RSL/Message.i.dfy
@@ -8,15 +8,15 @@ import opened AppStateMachine_i
 
 datatype RslMessage =
     RslMessage_Invalid()
-  | RslMessage_Request(seqno_req:int, val:AppMessage) //seqno_req可能作恶
+  | RslMessage_Request(seqno_req:int, val:AppMessage)
   | RslMessage_1a(bal_1a:Ballot)
-  | RslMessage_1b(bal_1b:Ballot, log_truncation_point:OperationNumber, votes:Votes) // log_truncation_point可能作恶
-  | RslMessage_2a(bal_2a:Ballot, opn_2a:OperationNumber, val_2a:RequestBatch) 
+  | RslMessage_1b(bal_1b:Ballot, log_truncation_point:OperationNumber, votes:Votes)
+  | RslMessage_2a(bal_2a:Ballot, opn_2a:OperationNumber, val_2a:RequestBatch)
   | RslMessage_2b(bal_2b:Ballot, opn_2b:OperationNumber, val_2b:RequestBatch)
-  | RslMessage_Heartbeat(bal_heartbeat:Ballot, suspicious:bool, opn_ckpt:OperationNumber) // suspicious，opn_ckpt可能作恶，suspicious作恶没关系，因为需要2f+1才触发选主，opn作恶好像也没关系，因为是选2f+1的地方做truncate的
+  | RslMessage_Heartbeat(bal_heartbeat:Ballot, suspicious:bool, opn_ckpt:OperationNumber)
   | RslMessage_Reply(seqno_reply:int, reply:AppMessage)
-  | RslMessage_AppStateRequest(bal_state_req:Ballot, opn_state_req:OperationNumber) 
+  | RslMessage_AppStateRequest(bal_state_req:Ballot, opn_state_req:OperationNumber)
   | RslMessage_AppStateSupply(bal_state_supply:Ballot, opn_state_supply:OperationNumber, app_state:AppState, reply_cache:ReplyCache)
-  | RslMessage_StartingPhase2(bal_2:Ballot, logTruncationPoint_2:OperationNumber) // logTruncationPoint_2可能作恶
+  | RslMessage_StartingPhase2(bal_2:Ballot, logTruncationPoint_2:OperationNumber)
 
 } 
