asset/final/spec/RSL/StateMachine.i.dfy
@@ -12,7 +12,8 @@ function HandleRequest(state:AppState, request:Request) : (AppState, Reply)
   (new_state, Reply(request.client, request.seqno, reply))
 }
 
-function {:opaque} HandleRequestBatchHidden(state:AppState, batch:RequestBatch) : (seq<AppState>, seq<Reply>)
+
+function HandleRequestBatchHidden(state:AppState, batch:RequestBatch) : (seq<AppState>, seq<Reply>)
   ensures var (states, replies) := HandleRequestBatchHidden(state, batch); 
           && |states| == |batch|+1
           && |replies| == |batch|
@@ -28,6 +29,8 @@ function {:opaque} HandleRequestBatchHidden(state:AppState, batch:RequestBatch) 
     (restStates+[new_state], restReplies+[Reply(batch[|batch|-1].client, batch[|batch|-1].seqno, reply)])
 }
 
+
+/*
 lemma{:timeLimitMultiplier 2} lemma_HandleRequestBatchHidden(state:AppState, batch:RequestBatch, states:seq<AppState>, replies:seq<Reply>)
   requires (states, replies) == HandleRequestBatchHidden(state, batch);
   ensures  && states[0] == state
@@ -103,23 +106,7 @@ lemma lemma_HandleRequestBatchTriggerHappy(state:AppState, batch:RequestBatch, s
   assert (states, replies) == HandleRequestBatchHidden(state, batch);
   lemma_HandleRequestBatchHidden(state, batch, states, replies);
 }
-
-// function HandleRequestBatch(state:AppState, batch:RequestBatch) : (seq<AppState>, seq<Reply>)
-// //  ensures var (states, replies) := HandleRequestBatch(state, batch); 
-// //          && states[0] == state
-// //          && |states| == |batch|+1 
-// //          && |replies| == |batch|
-// //          && (forall i :: 0 <= i < |batch| ==>
-// //                   && replies[i].Reply? 
-// //                   && ((states[i+1], replies[i].reply) == AppHandleRequest(states[i], batch[i].request))
-// //                   && replies[i].client == batch[i].client
-// //                   && replies[i].seqno == batch[i].seqno)
-// {
-//    var (states, replies) := HandleRequestBatchHidden(state, batch); 
-//    lemma_HandleRequestBatchHidden(state, batch, states, replies);
-//    (states, replies)
-// }
-
+*/
 
 function HandleRequestBatch(state:AppState, batch:RequestBatch) : (seq<AppState>, seq<Reply>)
  ensures var (states, replies) := HandleRequestBatch(state, batch); 
@@ -133,7 +120,7 @@ function HandleRequestBatch(state:AppState, batch:RequestBatch) : (seq<AppState>
                   && replies[i].seqno == batch[i].seqno)
 {
    var (states, replies) := HandleRequestBatchHidden(state, batch); 
-   lemma_HandleRequestBatchHidden(state, batch, states, replies);
+  //  lemma_HandleRequestBatchHidden(state, batch, states, replies); /* Manually commented */
    (states, replies)
 }
 
