asset/final/spec/RSL/Types.i.dfy
@@ -3,56 +3,58 @@ include "../Common/NodeIdentity.i.dfy"
 
 module LiveRSL__Types_i {
 
-import opened AppStateMachine_i
-import opened Concrete_NodeIdentity_i
+  import opened AppStateMachine_i
+  import opened Concrete_NodeIdentity_i
 
-type OperationNumber = int
-datatype Ballot = Ballot(seqno:int, proposer_id:int)
-    
-datatype Request = Request(client:NodeIdentity, seqno:int, request:AppMessage)
-datatype Reply = Reply(client:NodeIdentity, seqno:int, reply:AppMessage)
+  type OperationNumber = int
+  datatype Ballot = Ballot(seqno:int, proposer_id:int)
 
-type RequestBatch = seq<Request>
-type ReplyCache = map<NodeIdentity, Reply>
+  datatype Request = Request(client:NodeIdentity, seqno:int, request:AppMessage)
+  datatype Reply = Reply(client:NodeIdentity, seqno:int, reply:AppMessage)
 
-datatype Vote = Vote(max_value_bal:Ballot, ghost max_val:RequestBatch)
-type Votes = map<OperationNumber, Vote>
+  type RequestBatch = seq<Request>
+  type ReplyCache = map<NodeIdentity, Reply>
 
-datatype LearnerTuple = LearnerTuple(received_2b_message_senders:set<NodeIdentity>, candidate_learned_value:RequestBatch)
-type LearnerState = map<OperationNumber, LearnerTuple>
+  datatype Vote = Vote(max_value_bal:Ballot, /*ghost*/ max_val:RequestBatch)
+  type Votes = map<OperationNumber, Vote>
 
-predicate BalLt(ba:Ballot, bb:Ballot)
-{
-  || ba.seqno < bb.seqno
-  || (ba.seqno==bb.seqno && ba.proposer_id < bb.proposer_id)
-}
+  datatype LearnerTuple = LearnerTuple(received_2b_message_senders:set<NodeIdentity>, candidate_learned_value:RequestBatch)
+  type LearnerState = map<OperationNumber, LearnerTuple>
 
-predicate BalLeq(ba:Ballot, bb:Ballot)
-{
-  || ba.seqno < bb.seqno
-  || (ba.seqno==bb.seqno && ba.proposer_id <= bb.proposer_id)
-}
-
-lemma lemma_BalLtMiddle(ba:Ballot, bb:Ballot)
-  requires !BalLt(ba,bb)
-  requires ba!=bb
-  ensures BalLt(bb, ba)
-{
-}
-
-lemma lemma_BalLtProperties()
-  ensures forall ba,bb :: !BalLt(ba,bb) && ba!=bb ==> BalLt(bb,ba)
-  ensures forall ba,bb :: BalLeq(ba,bb) ==> BalLt(ba,bb) || ba==bb
-  // Transitivity
-  ensures forall ba,bb,bc :: BalLt(ba, bb) && BalLt(bb, bc) ==> BalLt(ba,bc)
-  ensures forall ba,bb,bc :: BalLt(ba, bb) && BalLeq(bb, bc) ==> BalLt(ba,bc)
-  ensures forall ba,bb,bc :: BalLeq(ba, bb) && BalLt(bb, bc) ==> BalLt(ba,bc)
-{
-  forall (ba,bb | !BalLt(ba,bb) && ba!=bb)
-    ensures BalLt(bb,ba)
+  predicate BalLt(ba:Ballot, bb:Ballot)
   {
-    lemma_BalLtMiddle(ba,bb);
+    || ba.seqno < bb.seqno
+    || (ba.seqno==bb.seqno && ba.proposer_id < bb.proposer_id)
   }
-}
 
-} 
+  predicate BalLeq(ba:Ballot, bb:Ballot)
+  {
+    || ba.seqno < bb.seqno
+    || (ba.seqno==bb.seqno && ba.proposer_id <= bb.proposer_id)
+  }
+
+  lemma lemma_BalLtMiddle(ba:Ballot, bb:Ballot)
+    requires !BalLt(ba,bb)
+    requires ba!=bb
+    ensures BalLt(bb, ba)
+  {
+  }
+
+  lemma lemma_BalLtProperties()
+    ensures forall ba,bb :: !BalLt(ba,bb) && ba!=bb ==> BalLt(bb,ba)
+    ensures forall ba,bb :: BalLeq(ba,bb) ==> BalLt(ba,bb) || ba==bb
+    // Transitivity
+    ensures forall ba,bb,bc :: BalLt(ba, bb) && BalLt(bb, bc) ==> BalLt(ba,bc)
+    ensures forall ba,bb,bc :: BalLt(ba, bb) && BalLeq(bb, bc) ==> BalLt(ba,bc)
+    ensures forall ba,bb,bc :: BalLeq(ba, bb) && BalLt(bb, bc) ==> BalLt(ba,bc)
+  {
+    /*
+    forall (ba,bb | !BalLt(ba,bb) && ba!=bb)
+      ensures BalLt(bb,ba)
+    {
+      lemma_BalLtMiddle(ba,bb);
+    }
+    */
+  }
+
+}
