asset/final/spec/SHT/Host.i.dfy
@@ -71,7 +71,7 @@ function DelegationMap_Init(rootIdentity:NodeIdentity) : DelegationMap {
     map k {:auto_trigger} :: rootIdentity
 }
 
-function method HashtableLookup(h:Hashtable, k:Key) : OptionalValue
+function /*method*/ HashtableLookup(h:Hashtable, k:Key) : OptionalValue
 {
     if k in h then ValuePresent(h[k]) else ValueAbsent()
 }
@@ -130,36 +130,6 @@ predicate Host_Init(s:Host, id:NodeIdentity, rootIdentity:NodeIdentity, hostIds:
     }
 
 // should be translated
-// predicate NextGetRequestReal(s:Host, s':Host, pkt:Packet, sm:SingleMessage, m:Message, out:set<Packet>, shouldSend:bool)
-//     requires pkt.msg.SingleMessage?
-//     requires pkt.msg.m.GetRequest?
-//     requires pkt.msg.m.k_getrequest in s.delegationMap
-//     ensures NextGetRequestReal(s,s',pkt,sm,m,out,shouldSend) ==>
-//             NextGetRequest_Reply(s,s',pkt.src,pkt.msg.seqno,pkt.msg.m.k_getrequest,sm,m,out,shouldSend) ==> 
-//             (exists sm1,m1,b :: NextGetRequest_Reply(s, s', pkt.src, pkt.msg.seqno, pkt.msg.m.k_getrequest, sm1, m1, out, b))
-//     ensures NextGetRequestReal(s,s',pkt,sm,m,out,shouldSend) ==>
-//             NextGetRequest(s,s',pkt,out)
-// {
-//     var k := pkt.msg.m.k_getrequest;
-//     var src := pkt.src;
-//     var seqno := pkt.msg.seqno;
-//     var owner := DelegateForKey(s.delegationMap, k);
-//     var newReceivedRequests := if owner == s.me then s.receivedRequests + [AppGetRequest(seqno, k)] else s.receivedRequests;
-//     var msg := if owner == s.me then Reply(k, HashtableLookup(s.h, k)) else Redirect(k, owner);
-
-//     && SendSingleMessageReal(s.sd, s'.sd, msg, src, sm, s.constants.params, shouldSend)
-//     // mode checking
-//     // shouldSend is output, but it is used as input
-//     && if ValidKey(k) && shouldSend then
-//         && m == msg
-//         && s' == s.(sd := s'.sd, receivedRequests := newReceivedRequests, receivedPacket := None)
-//         && out == {Packet(src, s.me, sm)}
-//        else
-//         && s' == s.(receivedPacket:=None)
-//         && m == msg
-//         && out == {}
-// }
-
 predicate NextGetRequestReal(s:Host, s':Host, pkt:Packet, sm:SingleMessage, m:Message, out:set<Packet>, shouldSend:bool)
     requires pkt.msg.SingleMessage?
     requires pkt.msg.m.GetRequest?
@@ -177,33 +147,63 @@ predicate NextGetRequestReal(s:Host, s':Host, pkt:Packet, sm:SingleMessage, m:Me
     var newReceivedRequests := if owner == s.me then s.receivedRequests + [AppGetRequest(seqno, k)] else s.receivedRequests;
     var msg := if owner == s.me then Reply(k, HashtableLookup(s.h, k)) else Redirect(k, owner);
 
-    var oldAckState := AckStateLookup(src, s.sd.sendState); 
-    var new_seqno := oldAckState.numPacketsAcked + |oldAckState.unAcked| + 1;
-    var temp_sm := SingleMessage(new_seqno, src, msg);
-
-    var (new_sd, new_sm, should_send) := if new_seqno > s.constants.params.max_seqno then
-        (s.sd, SingleMessage(0, src, msg), false)
-    else 
-        (s.sd.(sendState := s.sd.sendState[temp_sm.dst := oldAckState.(unAcked := oldAckState.unAcked + [temp_sm])]),
-        temp_sm,
-        true);
-    
-    && sm == new_sm
-    && shouldSend == should_send
-    && s'.sd == new_sd
-
-    // && SendSingleMessageReal(s.sd, s'.sd, msg, src, sm, s.constants.params, shouldSend)
+    && SendSingleMessageReal(s.sd, s'.sd, msg, src, sm, s.constants.params, shouldSend)
     // mode checking
     // shouldSend is output, but it is used as input
-    && if ValidKey(k) && should_send then
+    && if ValidKey(k) && shouldSend then
         && m == msg
         && s' == s.(sd := s'.sd, receivedRequests := newReceivedRequests, receivedPacket := None)
-        && out == {Packet(src, s.me, new_sm)}
+        && out == {Packet(src, s.me, sm)}
        else
         && s' == s.(receivedPacket:=None)
         && m == msg
         && out == {}
 }
+
+// predicate NextGetRequestReal(s:Host, s':Host, pkt:Packet, sm:SingleMessage, m:Message, out:set<Packet>, shouldSend:bool)
+//     requires pkt.msg.SingleMessage?
+//     requires pkt.msg.m.GetRequest?
+//     requires pkt.msg.m.k_getrequest in s.delegationMap
+//     ensures NextGetRequestReal(s,s',pkt,sm,m,out,shouldSend) ==>
+//             NextGetRequest_Reply(s,s',pkt.src,pkt.msg.seqno,pkt.msg.m.k_getrequest,sm,m,out,shouldSend) ==> 
+//             (exists sm1,m1,b :: NextGetRequest_Reply(s, s', pkt.src, pkt.msg.seqno, pkt.msg.m.k_getrequest, sm1, m1, out, b))
+//     ensures NextGetRequestReal(s,s',pkt,sm,m,out,shouldSend) ==>
+//             NextGetRequest(s,s',pkt,out)
+// {
+//     var k := pkt.msg.m.k_getrequest;
+//     var src := pkt.src;
+//     var seqno := pkt.msg.seqno;
+//     var owner := DelegateForKey(s.delegationMap, k);
+//     var newReceivedRequests := if owner == s.me then s.receivedRequests + [AppGetRequest(seqno, k)] else s.receivedRequests;
+//     var msg := if owner == s.me then Reply(k, HashtableLookup(s.h, k)) else Redirect(k, owner);
+
+//     var oldAckState := AckStateLookup(src, s.sd.sendState); 
+//     var new_seqno := oldAckState.numPacketsAcked + |oldAckState.unAcked| + 1;
+//     var temp_sm := SingleMessage(new_seqno, src, msg);
+
+//     var (new_sd, new_sm, should_send) := if new_seqno > s.constants.params.max_seqno then
+//         (s.sd, SingleMessage(0, src, msg), false)
+//     else 
+//         (s.sd.(sendState := s.sd.sendState[temp_sm.dst := oldAckState.(unAcked := oldAckState.unAcked + [temp_sm])]),
+//         temp_sm,
+//         true);
+    
+//     && sm == new_sm
+//     && shouldSend == should_send
+//     && s'.sd == new_sd
+
+//     // && SendSingleMessageReal(s.sd, s'.sd, msg, src, sm, s.constants.params, shouldSend)
+//     // mode checking
+//     // shouldSend is output, but it is used as input
+//     && if ValidKey(k) && should_send then
+//         && m == msg
+//         && s' == s.(sd := s'.sd, receivedRequests := newReceivedRequests, receivedPacket := None)
+//         && out == {Packet(src, s.me, new_sm)}
+//        else
+//         && s' == s.(receivedPacket:=None)
+//         && m == msg
+//         && out == {}
+// }
 
 
 
@@ -248,39 +248,6 @@ predicate NextSetRequest(s:Host, s':Host, pkt:Packet, out:set<Packet>)
 }
 
 // should be translated
-// predicate NextSetRequestReal(s:Host, s':Host, pkt:Packet, sm:SingleMessage, replym:Message, out:set<Packet>, shouldSend:bool)
-//     // requires DelegationMapComplete(s.delegationMap);
-//     requires pkt.msg.SingleMessage?
-//     requires pkt.msg.m.SetRequest?
-//     requires pkt.msg.m.k_setrequest in s.delegationMap
-//     ensures NextSetRequestReal(s,s',pkt,sm,replym,out,shouldSend) ==>
-//             NextSetRequest_Complete(s,s',pkt.src,pkt.msg.seqno,pkt.msg.m,sm,replym,out,shouldSend) ==>
-//             (exists sm1,m1,b1 :: NextSetRequest_Complete(s,s',pkt.src,pkt.msg.seqno,pkt.msg.m,sm1,m1,out,b1))
-//     ensures NextSetRequestReal(s,s',pkt,sm,replym,out,shouldSend) ==>
-//             NextSetRequest(s,s',pkt,out)
-// {
-//     var k := pkt.msg.m.k_setrequest;
-//     var ov := pkt.msg.m.v_setrequest;
-//     var seqno := pkt.msg.seqno;
-//     var src := pkt.src;
-//     var owner := DelegateForKey(s.delegationMap, k);
-//     var newhtable := if owner == s.me then (if ov.ValueAbsent? then mapremove(s.h, k) else s.h[k:=ov.v]) else s.h;
-//     var msg := if owner == s.me then Reply(k, ov) else Redirect(k, owner);
-//     var reqs := if owner == s.me then s.receivedRequests + [AppSetRequest(seqno, k, ov)] else s.receivedRequests;
-
-//     && SendSingleMessageReal(s.sd, s'.sd, msg, src, sm, s.constants.params, shouldSend)
-//     // mode checking
-//     // shouldSend is output, but it is used as input
-//     && if shouldSend && ValidKey(k) && ValidOptionalValue(ov) then
-//         && replym == msg
-//         && s' == s.(h := newhtable, sd := s'.sd, receivedRequests := reqs, receivedPacket := None)
-//         && out == {Packet(src, s.me, sm)}
-//     else
-//         && replym == msg
-//         && s' == s.(receivedPacket:=None)
-//         && out == {}
-// }
-
 predicate NextSetRequestReal(s:Host, s':Host, pkt:Packet, sm:SingleMessage, replym:Message, out:set<Packet>, shouldSend:bool)
     // requires DelegationMapComplete(s.delegationMap);
     requires pkt.msg.SingleMessage?
@@ -301,32 +268,65 @@ predicate NextSetRequestReal(s:Host, s':Host, pkt:Packet, sm:SingleMessage, repl
     var msg := if owner == s.me then Reply(k, ov) else Redirect(k, owner);
     var reqs := if owner == s.me then s.receivedRequests + [AppSetRequest(seqno, k, ov)] else s.receivedRequests;
 
-    var oldAckState := AckStateLookup(src, s.sd.sendState); 
-    var new_seqno := oldAckState.numPacketsAcked + |oldAckState.unAcked| + 1;
-    var temp_sm := SingleMessage(new_seqno, src, msg);
-
-    var (new_sd, new_sm, should_send) := if new_seqno > s.constants.params.max_seqno then
-        (s.sd, SingleMessage(0, src, msg), false)
-    else 
-        (s.sd.(sendState := s.sd.sendState[temp_sm.dst := oldAckState.(unAcked := oldAckState.unAcked + [temp_sm])]),
-        temp_sm,
-        true);
-    && sm == new_sm
-    && shouldSend == should_send
-    && s'.sd == new_sd
-
-    // && SendSingleMessageReal(s.sd, s'.sd, msg, src, sm, s.constants.params, shouldSend)
+    && SendSingleMessageReal(s.sd, s'.sd, msg, src, sm, s.constants.params, shouldSend)
     // mode checking
     // shouldSend is output, but it is used as input
-    && if should_send && ValidKey(k) && ValidOptionalValue(ov) then
+    && if shouldSend && ValidKey(k) && ValidOptionalValue(ov) then
         && replym == msg
         && s' == s.(h := newhtable, sd := s'.sd, receivedRequests := reqs, receivedPacket := None)
-        && out == {Packet(src, s.me, new_sm)}
+        && out == {Packet(src, s.me, sm)}
     else
         && replym == msg
         && s' == s.(receivedPacket:=None)
         && out == {}
 }
+
+// predicate NextSetRequestReal(s:Host, s':Host, pkt:Packet, sm:SingleMessage, replym:Message, out:set<Packet>, shouldSend:bool)
+//     // requires DelegationMapComplete(s.delegationMap);
+//     requires pkt.msg.SingleMessage?
+//     requires pkt.msg.m.SetRequest?
+//     requires pkt.msg.m.k_setrequest in s.delegationMap
+//     ensures NextSetRequestReal(s,s',pkt,sm,replym,out,shouldSend) ==>
+//             NextSetRequest_Complete(s,s',pkt.src,pkt.msg.seqno,pkt.msg.m,sm,replym,out,shouldSend) ==>
+//             (exists sm1,m1,b1 :: NextSetRequest_Complete(s,s',pkt.src,pkt.msg.seqno,pkt.msg.m,sm1,m1,out,b1))
+//     ensures NextSetRequestReal(s,s',pkt,sm,replym,out,shouldSend) ==>
+//             NextSetRequest(s,s',pkt,out)
+// {
+//     var k := pkt.msg.m.k_setrequest;
+//     var ov := pkt.msg.m.v_setrequest;
+//     var seqno := pkt.msg.seqno;
+//     var src := pkt.src;
+//     var owner := DelegateForKey(s.delegationMap, k);
+//     var newhtable := if owner == s.me then (if ov.ValueAbsent? then mapremove(s.h, k) else s.h[k:=ov.v]) else s.h;
+//     var msg := if owner == s.me then Reply(k, ov) else Redirect(k, owner);
+//     var reqs := if owner == s.me then s.receivedRequests + [AppSetRequest(seqno, k, ov)] else s.receivedRequests;
+
+//     var oldAckState := AckStateLookup(src, s.sd.sendState); 
+//     var new_seqno := oldAckState.numPacketsAcked + |oldAckState.unAcked| + 1;
+//     var temp_sm := SingleMessage(new_seqno, src, msg);
+
+//     var (new_sd, new_sm, should_send) := if new_seqno > s.constants.params.max_seqno then
+//         (s.sd, SingleMessage(0, src, msg), false)
+//     else 
+//         (s.sd.(sendState := s.sd.sendState[temp_sm.dst := oldAckState.(unAcked := oldAckState.unAcked + [temp_sm])]),
+//         temp_sm,
+//         true);
+//     && sm == new_sm
+//     && shouldSend == should_send
+//     && s'.sd == new_sd
+
+//     // && SendSingleMessageReal(s.sd, s'.sd, msg, src, sm, s.constants.params, shouldSend)
+//     // mode checking
+//     // shouldSend is output, but it is used as input
+//     && if should_send && ValidKey(k) && ValidOptionalValue(ov) then
+//         && replym == msg
+//         && s' == s.(h := newhtable, sd := s'.sd, receivedRequests := reqs, receivedPacket := None)
+//         && out == {Packet(src, s.me, new_sm)}
+//     else
+//         && replym == msg
+//         && s' == s.(receivedPacket:=None)
+//         && out == {}
+// }
 
 
 // should not translate
@@ -369,9 +369,10 @@ predicate NextDelegateReal(s:Host, s':Host, pkt:Packet, out:set<Packet>)
         && s'.numDelegations == s.numDelegations
        )
     && out == {}
-    && s'.sd == s.sd
-    && s'.receivedRequests == s.receivedRequests
-    && s'.receivedPacket == None
+    // && s'.sd == s.sd
+    // && s'.receivedRequests == s.receivedRequests
+    // && s'.receivedPacket == None
+    && s' == s.(delegationMap := s'.delegationMap, h := s'.h, numDelegations := s'.numDelegations, receivedPacket := None)
 }
 
 // should not translate
@@ -414,47 +415,6 @@ predicate NextShard_Wrapper(s:Host, s':Host, pkt:Packet, out:set<Packet>)
 }
 
 // this action should be translated
-// predicate NextShardReal(s:Host, s':Host, pkt:Packet, out:set<Packet>, sm:SingleMessage, shouldSend:bool)
-//     requires pkt.msg.SingleMessage?
-//     requires pkt.msg.m.Shard?
-//     requires DelegateForKeyRangeIsHost(s.delegationMap, pkt.msg.m.kr, s.me)
-//     requires pkt.msg.m.recipient != s.me
-//     requires pkt.msg.m.recipient in s.constants.hostIds
-//     ensures NextShardReal(s,s',pkt,out,sm,shouldSend) &&  
-//             !(   pkt.msg.m.recipient == s.me
-//            || !ValidKeyRange(pkt.msg.m.kr)
-//            || EmptyKeyRange(pkt.msg.m.kr)
-//            || pkt.msg.m.recipient !in s.constants.hostIds 
-//            || !DelegateForKeyRangeIsHost(s.delegationMap, pkt.msg.m.kr, s.me)
-//            || |ExtractRange(s.h, pkt.msg.m.kr)| >= max_hashtable_size()) ==> 
-//             NextShard(s,s',out,pkt.msg.m.kr,pkt.msg.m.recipient,sm,shouldSend) ==>
-//             NextShard_Wrapper(s,s',pkt,out)
-//     ensures NextShardReal(s,s',pkt,out,sm,shouldSend) ==>
-//             NextShard_Wrapper(s,s',pkt,out)
-// {
-//     var kr := pkt.msg.m.kr;
-//     var recipient := pkt.msg.m.recipient;
-//     && if (   pkt.msg.m.recipient == s.me
-//            || !ValidKeyRange(pkt.msg.m.kr)
-//            || EmptyKeyRange(pkt.msg.m.kr)
-//            || pkt.msg.m.recipient !in s.constants.hostIds 
-//            || !DelegateForKeyRangeIsHost(s.delegationMap, pkt.msg.m.kr, s.me)
-//            || |ExtractRange(s.h, pkt.msg.m.kr)| >= max_hashtable_size()) then
-//            // saturation check 
-//            // sm is not assigned here
-//             s' == s.(receivedPacket := None) && out == {}
-//         else
-//             && SendSingleMessageReal(s.sd, s'.sd, Delegate(kr, ExtractRange(s.h, kr)), recipient, sm, s.constants.params, shouldSend)
-//             // mode checking
-//             // shouldSend is output, but it is used as input
-//             && if shouldSend then
-//                 && out == { Packet(recipient, s.me, sm) }
-//                 && s' == s.(h := BulkRemoveHashtable(s.h, kr), delegationMap := UpdateDelegationMap(s.delegationMap, kr, recipient), sd := s'.sd, numDelegations := s.numDelegations + 1, receivedPacket := None)
-//             else
-//                 && out == {}
-//                 && s' == s.(numDelegations := s.numDelegations + 1, receivedPacket := None)
-// }
-
 predicate NextShardReal(s:Host, s':Host, pkt:Packet, out:set<Packet>, sm:SingleMessage, shouldSend:bool)
     requires pkt.msg.SingleMessage?
     requires pkt.msg.m.Shard?
@@ -475,48 +435,90 @@ predicate NextShardReal(s:Host, s':Host, pkt:Packet, out:set<Packet>, sm:SingleM
 {
     var kr := pkt.msg.m.kr;
     var recipient := pkt.msg.m.recipient;
-
     && if (   pkt.msg.m.recipient == s.me
            || !ValidKeyRange(pkt.msg.m.kr)
            || EmptyKeyRange(pkt.msg.m.kr)
            || pkt.msg.m.recipient !in s.constants.hostIds 
            || !DelegateForKeyRangeIsHost(s.delegationMap, pkt.msg.m.kr, s.me)
            || |ExtractRange(s.h, pkt.msg.m.kr)| >= max_hashtable_size()) then
-
-           
            // saturation check 
            // sm is not assigned here
+            && sm ==  CInvalidMessage() && shouldSend == true &&
             s' == s.(receivedPacket := None) && out == {}
         else
-            var src := recipient;
-            var msg := Delegate(kr, ExtractRange(s.h, kr));
-            var oldAckState := AckStateLookup(src, s.sd.sendState); 
-            var new_seqno := oldAckState.numPacketsAcked + |oldAckState.unAcked| + 1;
-            var temp_sm := SingleMessage(new_seqno, src, msg);
-
-            var (new_sd, new_sm, should_send) := if new_seqno > s.constants.params.max_seqno then
-                (s.sd, SingleMessage(0, src, msg), false)
-            else 
-                (s.sd.(sendState := s.sd.sendState[temp_sm.dst := oldAckState.(unAcked := oldAckState.unAcked + [temp_sm])]),
-                temp_sm,
-                true);
-
-            && sm == new_sm
-            && shouldSend == should_send
-            && s'.sd == new_sd
-
-            // && SendSingleMessageReal(s.sd, s'.sd, Delegate(kr, ExtractRange(s.h, kr)), recipient, sm, s.constants.params, shouldSend)
+            && SendSingleMessageReal(s.sd, s'.sd, Delegate(kr, ExtractRange(s.h, kr)), recipient, sm, s.constants.params, shouldSend)
             // mode checking
             // shouldSend is output, but it is used as input
-            && if should_send then
-                && out == { Packet(recipient, s.me, new_sm) }
+            && if shouldSend then
+                && out == { Packet(recipient, s.me, sm) }
                 && s' == s.(h := BulkRemoveHashtable(s.h, kr), delegationMap := UpdateDelegationMap(s.delegationMap, kr, recipient), sd := s'.sd, numDelegations := s.numDelegations + 1, receivedPacket := None)
             else
                 && out == {}
                 && s' == s.(numDelegations := s.numDelegations + 1, receivedPacket := None)
 }
 
-function method max_hashtable_size():int { 62 }
+// predicate NextShardReal(s:Host, s':Host, pkt:Packet, out:set<Packet>, sm:SingleMessage, shouldSend:bool)
+//     requires pkt.msg.SingleMessage?
+//     requires pkt.msg.m.Shard?
+//     requires DelegateForKeyRangeIsHost(s.delegationMap, pkt.msg.m.kr, s.me)
+//     requires pkt.msg.m.recipient != s.me
+//     requires pkt.msg.m.recipient in s.constants.hostIds
+//     ensures NextShardReal(s,s',pkt,out,sm,shouldSend) &&  
+//             !(   pkt.msg.m.recipient == s.me
+//            || !ValidKeyRange(pkt.msg.m.kr)
+//            || EmptyKeyRange(pkt.msg.m.kr)
+//            || pkt.msg.m.recipient !in s.constants.hostIds 
+//            || !DelegateForKeyRangeIsHost(s.delegationMap, pkt.msg.m.kr, s.me)
+//            || |ExtractRange(s.h, pkt.msg.m.kr)| >= max_hashtable_size()) ==> 
+//             NextShard(s,s',out,pkt.msg.m.kr,pkt.msg.m.recipient,sm,shouldSend) ==>
+//             NextShard_Wrapper(s,s',pkt,out)
+//     ensures NextShardReal(s,s',pkt,out,sm,shouldSend) ==>
+//             NextShard_Wrapper(s,s',pkt,out)
+// {
+//     var kr := pkt.msg.m.kr;
+//     var recipient := pkt.msg.m.recipient;
+
+//     && if (   pkt.msg.m.recipient == s.me
+//            || !ValidKeyRange(pkt.msg.m.kr)
+//            || EmptyKeyRange(pkt.msg.m.kr)
+//            || pkt.msg.m.recipient !in s.constants.hostIds 
+//            || !DelegateForKeyRangeIsHost(s.delegationMap, pkt.msg.m.kr, s.me)
+//            || |ExtractRange(s.h, pkt.msg.m.kr)| >= max_hashtable_size()) then
+
+           
+//            // saturation check 
+//            // sm is not assigned here
+//             s' == s.(receivedPacket := None) && out == {}
+//         else
+//             var src := recipient;
+//             var msg := Delegate(kr, ExtractRange(s.h, kr));
+//             var oldAckState := AckStateLookup(src, s.sd.sendState); 
+//             var new_seqno := oldAckState.numPacketsAcked + |oldAckState.unAcked| + 1;
+//             var temp_sm := SingleMessage(new_seqno, src, msg);
+
+//             var (new_sd, new_sm, should_send) := if new_seqno > s.constants.params.max_seqno then
+//                 (s.sd, SingleMessage(0, src, msg), false)
+//             else 
+//                 (s.sd.(sendState := s.sd.sendState[temp_sm.dst := oldAckState.(unAcked := oldAckState.unAcked + [temp_sm])]),
+//                 temp_sm,
+//                 true);
+
+//             && sm == new_sm
+//             && shouldSend == should_send
+//             && s'.sd == new_sd
+
+//             // && SendSingleMessageReal(s.sd, s'.sd, Delegate(kr, ExtractRange(s.h, kr)), recipient, sm, s.constants.params, shouldSend)
+//             // mode checking
+//             // shouldSend is output, but it is used as input
+//             && if should_send then
+//                 && out == { Packet(recipient, s.me, new_sm) }
+//                 && s' == s.(h := BulkRemoveHashtable(s.h, kr), delegationMap := UpdateDelegationMap(s.delegationMap, kr, recipient), sd := s'.sd, numDelegations := s.numDelegations + 1, receivedPacket := None)
+//             else
+//                 && out == {}
+//                 && s' == s.(numDelegations := s.numDelegations + 1, receivedPacket := None)
+// }
+
+function /*method*/ max_hashtable_size():int { 62 }
 
 
 
@@ -543,13 +545,13 @@ predicate NextReplyReal(s:Host, s':Host, pkt:Packet, out:set<Packet>)
 }
 
 // should not translate
-predicate NextRedirect(s:Host, s':Host, pkt:Packet, out:set<Packet>)
-    requires pkt.msg.SingleMessage?
-{
-       pkt.msg.m.Redirect?
-    && out == {}
-    && s' == s.(receivedPacket := None)
-}
+// predicate NextRedirect(s:Host, s':Host, pkt:Packet, out:set<Packet>)
+//     requires pkt.msg.SingleMessage?
+// {
+//        pkt.msg.m.Redirect?
+//     && out == {}
+//     && s' == s.(receivedPacket := None)
+// }
 
 // should be translated
 predicate NextRedirectReal(s:Host, s':Host, pkt:Packet, out:set<Packet>)
@@ -570,65 +572,65 @@ predicate ShouldProcessReceivedMessage(s:Host)
  && ((s.receivedPacket.v.msg.m.Delegate? || s.receivedPacket.v.msg.m.Shard?) ==> s.numDelegations < s.constants.params.max_delegations - 2)
 }
 
-predicate Process_Message(s:Host, s':Host, out:set<Packet>)
-    requires DelegationMapComplete(s.delegationMap)
-    // requires s.receivedPacket.v.msg.m.GetRequest? ==> s.receivedPacket.v.msg.m.k_getrequest in s.delegationMap
-    // requires s.receivedPacket.v.msg.m.SetRequest? ==> s.receivedPacket.v.msg.m.k_setrequest in s.delegationMap
-{
-    if ShouldProcessReceivedMessage(s) then
-           (NextGetRequest(s, s', s.receivedPacket.v, out)
-        || NextSetRequest(s, s', s.receivedPacket.v, out)
-        || NextDelegate(s, s', s.receivedPacket.v, out)
-        || NextShard_Wrapper(s, s', s.receivedPacket.v, out)
-        || NextReply(s, s', s.receivedPacket.v, out)
-        || NextRedirect(s, s', s.receivedPacket.v, out))
-         && s'.receivedPacket.None?
-    else
-        s' == s && out == {}
-}
+// predicate Process_Message(s:Host, s':Host, out:set<Packet>)
+//     requires DelegationMapComplete(s.delegationMap)
+//     // requires s.receivedPacket.v.msg.m.GetRequest? ==> s.receivedPacket.v.msg.m.k_getrequest in s.delegationMap
+//     // requires s.receivedPacket.v.msg.m.SetRequest? ==> s.receivedPacket.v.msg.m.k_setrequest in s.delegationMap
+// {
+//     if ShouldProcessReceivedMessage(s) then
+//            (NextGetRequest(s, s', s.receivedPacket.v, out)
+//         || NextSetRequest(s, s', s.receivedPacket.v, out)
+//         || NextDelegate(s, s', s.receivedPacket.v, out)
+//         || NextShard_Wrapper(s, s', s.receivedPacket.v, out)
+//         || NextReply(s, s', s.receivedPacket.v, out)
+//         || NextRedirect(s, s', s.receivedPacket.v, out))
+//          && s'.receivedPacket.None?
+//     else
+//         s' == s && out == {}
+// }
 
-predicate ReceivePacket(s:Host, s':Host, pkt:Packet, out:set<Packet>, ack:Packet)
-{
-    if s.receivedPacket.None? then    // No packet currently waiting to be processed
-        && ReceiveSingleMessage(s.sd, s'.sd, pkt, ack, out) // Record and possibly ack it
-        // && pkt.msg.SingleMessage? && ShouldAckSingleMessage(s.sd,pkt) ==> var m := Ack(pkt.msg.seqno); ack == Packet(dst:=pkt.src, src:=pkt.dst, msg:=m)
-        && (if NewSingleMessage(s.sd, pkt) then
-               s'.receivedPacket == Some(pkt)   // Enqueue this packet for processing
-            else
-               s'.receivedPacket.None?)
-        && s' == s.(sd := s'.sd, receivedPacket := s'.receivedPacket)  // Nothing else changes
-    else 
-        s' == s && out == {}
-}
+// predicate ReceivePacket(s:Host, s':Host, pkt:Packet, out:set<Packet>, ack:Packet)
+// {
+//     if s.receivedPacket.None? then    // No packet currently waiting to be processed
+//         && ReceiveSingleMessage(s.sd, s'.sd, pkt, ack, out) // Record and possibly ack it
+//         // && pkt.msg.SingleMessage? && ShouldAckSingleMessage(s.sd,pkt) ==> var m := Ack(pkt.msg.seqno); ack == Packet(dst:=pkt.src, src:=pkt.dst, msg:=m)
+//         && (if NewSingleMessage(s.sd, pkt) then
+//                s'.receivedPacket == Some(pkt)   // Enqueue this packet for processing
+//             else
+//                s'.receivedPacket.None?)
+//         && s' == s.(sd := s'.sd, receivedPacket := s'.receivedPacket)  // Nothing else changes
+//     else 
+//         s' == s && out == {}
+// }
 
 
-predicate ProcessReceivedPacket(s:Host, s':Host, out:set<Packet>)
-    requires DelegationMapComplete(s.delegationMap)
-{
-    if s.receivedPacket.Some? then 
-        Process_Message(s, s', out)
-    else
-        s' == s && out == {}
-}
+// predicate ProcessReceivedPacket(s:Host, s':Host, out:set<Packet>)
+//     requires DelegationMapComplete(s.delegationMap)
+// {
+//     if s.receivedPacket.Some? then 
+//         Process_Message(s, s', out)
+//     else
+//         s' == s && out == {}
+// }
 
 // REVIEW: For safety, we don't need to retransmit at all.  
 // We could also just retransmit some, but not all, leaving it to the impl to decide.
 // For liveness, we have to retransmit some, and at the very least, retransmit in some order.
 // I suspect retransmitting them all will simplify things, however.
-predicate SpontaneouslyRetransmit(s:Host, s':Host, out:set<Packet>)
-{
-    (out == UnAckedMessages(s.sd, s.me) && s == s')
-}
+// predicate SpontaneouslyRetransmit(s:Host, s':Host, out:set<Packet>)
+// {
+//     (out == UnAckedMessages(s.sd, s.me) && s == s')
+// }
 
-predicate Host_Next(s:Host, s':Host, recv:set<Packet>, out:set<Packet>)
-{
-       s'.constants == s.constants
-    && s'.me == s.me
-    && DelegationMapComplete(s.delegationMap)
-    && (
-           (exists pkt, ack :: pkt in recv && ReceivePacket(s, s', pkt, out, ack))
-        || ProcessReceivedPacket(s, s', out)
-        || SpontaneouslyRetransmit(s, s', out)
-       )
-}
+// predicate Host_Next(s:Host, s':Host, recv:set<Packet>, out:set<Packet>)
+// {
+//        s'.constants == s.constants
+//     && s'.me == s.me
+//     && DelegationMapComplete(s.delegationMap)
+//     && (
+//            (exists pkt, ack :: pkt in recv && ReceivePacket(s, s', pkt, out, ack))
+//         || ProcessReceivedPacket(s, s', out)
+//         || SpontaneouslyRetransmit(s, s', out)
+//        )
+// }
 } 
